verifier

programs/Programs/Simple/ReverseInplace/module.wat
@@ -1,0 +1,68 @@
+(module
+  (type (;0;) (func (param i32 i32)))
+  (table (;0;) 1 1 funcref)
+  (memory (;0;) 16)
+  (global (;0;) (mut i32) i32.const 1048576)
+  (global (;1;) i32 i32.const 1048576)
+  (global (;2;) i32 i32.const 1048576)
+  (export "memory" (memory 0))
+  (export "reverse_inplace" (func 0))
+  (export "__data_end" (global 1))
+  (export "__heap_base" (global 2))
+  (func (;0;) (type 0) (param i32 i32)
+    (local i32 i32 i32)
+    block ;; label = @1
+      local.get 1
+      i32.const 2
+      i32.lt_u
+      br_if 0 (;@1;)
+      local.get 1
+      i32.const -1
+      i32.add
+      local.set 2
+      local.get 1
+      i32.const 2
+      i32.shl
+      local.get 0
+      i32.add
+      i32.const -4
+      i32.add
+      local.set 1
+      i32.const 1
+      local.set 3
+      loop ;; label = @2
+        local.get 0
+        i32.load
+        local.set 4
+        local.get 0
+        local.get 1
+        i32.load
+        i32.store
+        local.get 1
+        local.get 4
+        i32.store
+        local.get 0
+        i32.const 4
+        i32.add
+        local.set 0
+        local.get 1
+        i32.const -4
+        i32.add
+        local.set 1
+        local.get 3
+        local.get 2
+        i32.const -1
+        i32.add
+        local.tee 2
+        i32.lt_u
+        local.set 4
+        local.get 3
+        i32.const 1
+        i32.add
+        local.set 3
+        local.get 4
+        br_if 0 (;@2;)
+      end
+    end
+  )
+)
