verifier/template/rust/is_even/src/lib.rs
@@ -1,0 +1,5 @@
+mod exports;
+
+pub fn is_even(n: i32) -> bool {
+    n % 2 == 0
+}
