verifier/template/rust/is_odd/src/lib.rs
@@ -1,0 +1,5 @@
+mod exports;
+
+pub fn is_odd(n: i32) -> bool {
+    !is_even::is_even(n)
+}
