verifier/template/lean/Project/IsEven/Proof.lean
@@ -1,0 +1,15 @@
+import Project.IsEven.Spec
+
+namespace Project.IsEven.Proof
+
+open Wasm Project.IsEven Project.IsEven.Spec
+
+theorem is_even_spec : IsEvenSpec := by
+  intro initial n
+  apply TerminatesWith.of_wp_entry_wat
+    (f := ⟨[.i32], [], func0, some [.i32]⟩) rfl rfl
+  unfold func0
+  wp_run
+  simp [UInt32.and_one_eq_zero_iff_toNat_mod_two, UInt32.and_comm]
+
+end Project.IsEven.Proof
